case_study/RiscvPmp/Machine.v
@@ -1464,7 +1464,9 @@ Module Import RiscvPmpProgram <: Program RiscvPmpBase.
       let (μupd,readv) := fun_read_mmio μ width addr in
       (γ' , μ' , res) = (γ , μupd , inr readv);
     ForeignCall (@mmio_write width H) [addr; data] res γ γ' μ μ' :=
-      (γ' , μ' , res) = (γ , @fun_write_mmio μ width addr data , inr true);
+      let (power, μ'') := @fun_handle_write_mmio μ width addr data in
+      let res' := if power then inr true else inl "Shutdown" in
+      (γ' , μ' , res) = (γ , μ'', res');
     ForeignCall (@within_mmio width H) [addr] res γ γ' μ μ' :=
       (γ' , μ' , res) = (γ , μ , inr (fun_within_mmio width addr));
     ForeignCall decode [code] res γ γ' μ μ' :=
@@ -1478,7 +1480,7 @@ Module Import RiscvPmpProgram <: Program RiscvPmpBase.
   Local Arguments ForeignCall {_ _} f /.
   Lemma ForeignProgress {σs σ} (f : 𝑭𝑿 σs σ) (args : NamedEnv Val σs) γ μ :
     exists γ' μ' res, ForeignCall f args res γ γ' μ μ'.
-  Proof. destruct f; env.destroy args; [| | cbn; destruct fun_read_mmio|..]; repeat econstructor.
+  Proof. destruct f; env.destroy args; [| | cbn; destruct fun_read_mmio | cbn; repeat case_match | ..]; repeat econstructor.
   Qed.
   End ForeignKit.
 
